refinedVST/typing/array.v
@@ -1,0 +1,648 @@
+From iris.algebra Require Import list.
+From VST.typing Require Export type.
+(* From VST.typing Require Import programs singleton bytes int own.
+From VST.typing Require Import type_options. *)
+From VST.floyd Require Import aggregate_pred.
+Import aggregate_pred.
+From VST.floyd Require Export field_at.
+Section array.
+
+  Context `{!typeG OK_ty Σ} {cs : compspecs}.
+
+  Lemma array_pred_shift_addr: forall {A}{d: Inhabitant A} (lo hi lo' hi' mv : Z) (P: Z -> A -> val -> mpred) (v: list A) (p p':address) (cty:Ctypes.type),
+    lo - lo' = mv ->
+    hi - hi' = mv ->
+    p' = (p.1, p.2 + mv * expr.sizeof cty) ->
+    (forall i i', lo <= i < hi -> i - i' = mv -> P i' (Znth (i' - lo') v) p' = P i (Znth (i - lo) v) p) ->
+    array_pred lo' hi' P v p' = array_pred lo hi P v p.
+  Proof.
+    intros.
+    unfold array_pred, floyd.aggregate_pred.array_pred.
+    f_equal; first by f_equal; apply prop_ext; lia.
+    replace (hi' - lo') with (hi - lo) by lia.
+    destruct (zlt hi lo).
+    - rewrite -> Z2Nat_neg by lia. reflexivity.
+    - apply rangespec_shift; intros.
+      rewrite (H2 i' i); try lia. done.
+  Qed.
+
+  Ltac unfold_mapsto := 
+    rewrite /heap_mapsto_own_state_type /heap_mapsto_own_state /mapsto.
+
+  Lemma value_fits_array_app s1 s2 s3 cty v1 v2 v:
+    0 <= s1 ->
+    0 <= s2 ->
+    s3 = s1 + s2 ->
+    v = v1 ++ v2 ->
+    value_fits (tarray cty $ s1) v1 ->
+    value_fits (tarray cty $ s2) v2 ->
+    value_fits (tarray cty $ s3) v.
+  Proof.
+    intros ?? -> -> [hd1 hd2] [ts1 ts2].
+    split.
+    - rewrite /unfold_reptype /= in hd1 ts1.
+      rewrite /unfold_reptype Zlength_app hd1 ts1 /=.
+      rewrite -!Z2Nat_id' /=.
+      lia.
+    - rewrite Forall_app.
+      split; done.
+  Qed.
+
+  Lemma array_split l l_1 (s s1 s2:Z) cty v v_hd v_tl :
+    v = v_hd ++ v_tl ->
+    1 <= s1 ->
+    s1 = Zlength v_hd ->
+    s2 = Zlength v_tl ->
+    s = s1 + s2 ->
+    l_1 = (l.1, l.2 + s1 * @expr.sizeof cs cty) ->
+    l ↦[Own]|tarray cty s| v ⊣⊢
+    l ↦[Own]|tarray cty s1| v_hd ∗
+    l_1 ↦[Own]|tarray cty s2| v_tl.
+  Proof.
+    intros Hv ? Hs1 Hs2 Hs Hl.
+    unfold_mapsto.
+    apply (pure_equiv _  _ (value_fits (tarray cty s) (v_hd++v_tl))).
+    { rewrite Hv.
+      apply data_at_rec_value_fits. }
+    { iDestruct 1 as "(↦hd & ↦tl)".
+      iPoseProof (data_at_rec_value_fits with "↦hd") as "%v_fits1".
+      iPoseProof (data_at_rec_value_fits with "↦tl") as "%v_fits2".
+      iPureIntro.
+      eapply value_fits_array_app; [..|apply v_fits1|apply v_fits2].
+      all: try done; try rep_lia.
+    }
+    intros [v_fits _].
+    rewrite data_at_rec_eq /=.
+    rewrite (split_array_pred _ s1); try rep_lia.
+    2: { rewrite Hv v_fits; lia. }
+    
+    rewrite data_at_rec_eq /unfold_reptype /=.
+    assert (sublist 0 s1 v = v_hd) as Hsub1.
+    { rewrite Hv Hs1 sublist0_app1; last rep_lia.
+      rewrite sublist_same //.
+    }
+    assert (sublist s1 s v = v_tl) as Hsub2.
+    { rewrite Hv sublist_app2; last rep_lia.
+      rewrite Hs1 sublist_same //; rep_lia.
+    }
+    rewrite !Z.sub_0_r !Z.max_r; [|rep_lia..].
+    rewrite Hsub1 Hsub2.
+    f_equiv.
+    rewrite [in X in _ ⊣⊢ X ]/data_at_rec /unfold_reptype /= .
+    apply seplog_tactics.eq_equiv.
+    (* rewrite Hv.
+    assert (0 < s) as Hs' by rep_lia. *)
+    rewrite !Z.max_r; [|rep_lia..].
+    erewrite (array_pred_shift_addr s1 s 0 s2 s1 ); try lia; try done.
+    intros i i' _ Hi.
+    assert (i'=i-s1) as -> by lia.
+    rewrite !mapsto_memory_block.at_offset_eq Hl.
+    f_equal.
+    - f_equal. lia.
+    - rewrite /offset_val /= !ptrofs_add_repr.
+      do 2 f_equal. lia.
+  Qed.
+
+  Lemma array_split_ext l l_1 (s s1 s2:Z) cty :
+    1 <= s1 ->
+    0 <= s2 ->
+    s = s1 + s2 ->
+    l_1 = (l.1, l.2 + s1 * @expr.sizeof cs cty) ->
+    l ↦[Own]|tarray cty s| ⊣⊢
+    l ↦[Own]|tarray cty s1| ∗
+    l_1 ↦[Own]|tarray cty s2|.
+  Proof.
+    intros ?? -> Hl.
+    iSplit.
+    - iDestruct 1 as (v) "↦".
+      iPoseProof (data_at_rec_value_fits with "↦") as "%v_fits".
+      destruct v_fits as [v_fits _].
+      rewrite /unfold_reptype Z.max_r /= in v_fits; [|rep_lia].
+      rewrite (array_split _ _ _ _ _ _ _ (sublist 0 s1 v) (sublist s1 (s1+s2) v)) //.
+      2: { rewrite sublist_rejoin; try rep_lia.
+           - rewrite sublist_same //.
+           - rewrite v_fits; rep_lia. }
+      2: { rewrite Zlength_sublist; try rep_lia. rewrite v_fits; rep_lia. }
+      2: { rewrite Zlength_sublist; try rep_lia. rewrite v_fits; rep_lia. }
+      iDestruct "↦" as "[↦hd ↦tl]".
+      rewrite Zlength_sublist; try rep_lia. 2: rewrite v_fits; rep_lia.
+      assert (s1 + s2 - s1 = s2) as -> by lia.
+      iSplitL "↦hd"; iExists _; done.
+    - iDestruct 1 as "[[%v1 ↦hd] [%v2 ↦tl]]".
+      iPoseProof (data_at_rec_value_fits with "↦hd") as "%v_fits1".
+      iPoseProof (data_at_rec_value_fits with "↦tl") as "%v_fits2".
+      destruct v_fits1 as [v_fits1 _].
+      destruct v_fits2 as [v_fits2 _].
+      rewrite /unfold_reptype !Z.max_r /= in v_fits1 v_fits2; [|rep_lia..].
+      iExists (v1 ++ v2).
+      rewrite (array_split _ _ _ _ _ _ (v1++v2) v1 v2); try done; try rep_lia.
+      iFrame.
+    Qed.
+
+  (* maybe something like array_pred? *)
+  Program Definition array (cty:Ctypes.type) (tys : list type) : type(cty:=tarray cty (length tys)) := {|
+    ty_has_op_type mt := False%type ;
+    ty_own β l := (
+      <affine> ⌜l `has_layout_loc` (tarray cty (length tys))⌝ ∗
+      ([∗ list] i ↦ ty ∈ tys,
+        (l.1, l.2 + nested_field_offset (tarray cty (length tys)) [ArraySubsc i])%Z ◁ₗ{β} ty) ∗
+      l ↦[ β ]| tarray cty (length tys) |
+      )%I
+    ;
+    ty_own_val rep_v :=
+      (
+        <affine> ⌜rep_v `has_layout_val` (tarray cty (length tys))⌝ ∗
+        [∗ list] v';ty ∈ rep_v;tys, (v' ◁ᵥ ty))%I;
+  |}.
+  Next Obligation.
+    iIntros (cty tys l E He) "($&Ha&%v&Hb)".
+    iSplitL "Ha".
+    - iApply big_sepL_fupd. iApply (big_sepL_impl with "Ha").
+      iIntros "!#" (???) "a".
+      by iApply ty_share.
+    - rewrite /heap_mapsto_own_state_type /heap_mapsto_own_state.
+      iExists v.
+      iApply inv_alloc. by iFrame.
+  Qed.
+  Next Obligation. by iIntros (cty tys mt l ?) "[% _]". Qed.
+  Next Obligation. by iIntros (cty tys mt v ?) "(?&_)". Qed.
+  Next Obligation.
+    move => cty tys mt l _. iIntros "[%l_has_layout_loc H]".
+    iInduction (tys) as [|ty tys] "IH" forall (l l_has_layout_loc); csimpl.
+    { iExists []. iSplitR => //. iSplitR => //. }
+    iDestruct "H" as "((tys_hd & tys_tl) & ↦)".
+    pose l_1:address := (l.1, l.2 + @expr.sizeof cs cty)%Z.
+    rewrite /heap_mapsto_own_state_type /heap_mapsto_own_state /mapsto.
+    iDestruct "↦" as (v) "↦".
+    iPoseProof (data_at_rec_value_fits with "↦") as "%v_fits".
+    destruct v_fits as [v_fits _].
+    destruct v eqn:Heqv; first done.
+    assert (0 `max` length tys = length tys) as Hlength_tys by lia.
+    
+    iAssert (
+             l ↦[Own]|(tarray cty 1)| ∗
+             l_1 ↦[Own]|(tarray cty ((length tys)))| )%I with "[↦]" as "[↦hd ↦tl]".
+    {
+      
+      rewrite -Heqv /= in v_fits.
+      rewrite data_at_rec_eq /=.
+      rewrite (split_array_pred _ 1).
+      2: { lia. }
+      2: { rewrite -Heqv //. }
+      iDestruct "↦" as "[↦hd ↦tl]".
+      iSplitL "↦hd".
+      { iFrame. }
+      rewrite -Heqv /l_1 /=.
+      iExists _.
+      rewrite /heap_mapsto_own_state_type /heap_mapsto_own_state /mapsto.
+      rewrite data_at_rec_eq /unfold_reptype /=.
+      assert (expr.sizeof cty = 1 * expr.sizeof cty) as -> by lia.
+
+      erewrite (array_pred_shift_addr 1 (1 + length tys)); try lia.
+      2: {
+        intros i i' _ Hi.
+        assert (i'=i-1) as -> by lia.
+        rewrite !mapsto_memory_block.at_offset_eq.
+        f_equal.
+        - f_equal. lia.
+        - rewrite /offset_val /= !ptrofs_add_repr.
+          do 2 f_equal. lia.
+      }
+      iClear "#".
+      iStopProof. f_equiv.
+      - lia.
+      - done. 
+    }
+
+    iDestruct ("IH" $! l_1 with "[] [tys_tl ↦tl]") as "(%v_rep_tl & ↦tl & % & tys_tl)"; iClear "IH".
+    {
+      clear -l_has_layout_loc Hlength_tys.
+      (* TODO this should be in rep_lia? *)
+      pose proof (sizeof_pos cty) as Hcty_size_pos.
+      iPureIntro.
+      rewrite /has_layout_loc /field_compatible in l_has_layout_loc.
+      destruct l_has_layout_loc as (? & ? & ? & ? & ?).
+      rewrite /has_layout_loc /field_compatible /l_1.
+      simpl in H1.
+      split3; try done.
+      split3; try done.
+      - rewrite /= Hlength_tys.
+        rewrite -ptrofs_add_repr /expr.sizeof.
+        destruct (Ptrofs.unsigned_add_either (Ptrofs.repr l.2) 
+                                             (Ptrofs.repr (sizeof cty))) as [-> | ->].
+        + rewrite [Ptrofs.unsigned (Ptrofs.repr (sizeof cty))]Ptrofs.unsigned_repr; rep_lia.
+        + rep_lia.
+      - rewrite /SeparationLogic.align_compatible /=.
+        rewrite -ptrofs_add_repr /expr.sizeof.
+        rewrite /SeparationLogic.align_compatible /= in H2.
+        pose proof (align_mem.align_compatible_rec_Tarray_inv _ _ _ _ _ H2).
+        rewrite Ptrofs.unsigned_add_carry.
+        rewrite /Ptrofs.add_carry.
+        if_tac.
+        + rewrite Ptrofs.unsigned_zero /= Z.mul_0_l Z.sub_0_r.
+          rewrite [Ptrofs.unsigned (Ptrofs.repr (sizeof cty))]Ptrofs.unsigned_repr; last rep_lia.
+          constructor. intros. rewrite -Z.add_assoc Zred_factor2. apply H4. lia.
+        + rewrite [Ptrofs.unsigned (Ptrofs.repr (sizeof cty))]Ptrofs.unsigned_repr in H5; last rep_lia.
+          rewrite Ptrofs.unsigned_zero Z.add_0_r in H5.
+          assert ( Ptrofs.unsigned (Ptrofs.repr l.2) + sizeof cty < Ptrofs.modulus) by rep_lia.
+          contradiction.
+    }
+    {
+      iClear "#".
+      iFrame.
+      iApply (big_sepL_impl with "tys_tl").
+      iIntros "!>" (i ty_i Hty_i) "?".
+      rewrite /nested_field_offset /=.
+      iStopProof. do 2 f_equiv. lia.
+    }
+     v.
+
+
+    { rewrite /nested_field_offset /l_1 /=. iStopProof. do 5 f_equiv. lia. }
+    iExists ()
+      
+    intros (?&?)%Forall_cons. csimpl.
+    rewrite offset_loc_0. iDestruct "Htys" as "[Hty Htys]".
+    iDestruct (loc_in_bounds_split_mul_S with "Hb") as "[Hb1 Hb2]".
+    iDestruct (ty_deref with "Hty") as (v') "[Hl Hty]"; [done|].
+    iDestruct (ty_size_eq with "Hty") as %Hszv; [done|].
+    setoid_rewrite offset_loc_S.
+    iDestruct ("IH" $! (l offset{ly}ₗ 1) with "[//] [Hb2] Htys") as (vs') "(Hl' & Hsz & Htys)".
+    { by rewrite /offset_loc Z.mul_1_r. }
+    iDestruct "Hsz" as %Hsz. iExists (v' ++ vs').
+    rewrite /has_layout_val heap_mapsto_app Hszv offset_loc_1 take_app_length' // drop_app_length' // length_app Hszv Hsz.
+    iFrame. iPureIntro. rewrite /ly_size/= -/(ly_size _). lia.
+  Qed.
+  Next Obligation.
+    move => ly tys ot mt l v [-> [? [? ]]]. iIntros (Hlys Hl) "Hl".
+    iDestruct 1 as (Hv) "Htys". iSplit => //.
+    iInduction (tys) as [|ty tys] "IH" forall (l v Hlys Hv Hl); csimpl in *.
+    { rewrite Nat.mul_0_r right_id. by iApply heap_mapsto_loc_in_bounds_0. }
+    move: Hlys. intros [? ?]%Forall_cons. iDestruct "Htys" as "[Hty Htys]".
+    rewrite -{1}(take_drop (ly_size ly) v).
+    rewrite offset_loc_0 heap_mapsto_app length_take_le ?Hv; last by repeat unfold ly_size => /=; lia.
+    iDestruct "Hl" as "[Hl Hl']".
+    iDestruct (heap_mapsto_loc_in_bounds with "Hl") as "#Hb1".
+    iDestruct (ty_ref with "[] Hl Hty") as "$" => //.
+    setoid_rewrite offset_loc_S. rewrite offset_loc_1.
+    iDestruct ("IH" with "[//] [] [] Hl' Htys") as "[#Hb2 $]".
+    { iPureIntro. rewrite /has_layout_val length_drop Hv. by repeat unfold ly_size => /=; lia. }
+    { iPureIntro. by apply has_layout_loc_ly_mult_offset. }
+    iApply loc_in_bounds_split_mul_S. rewrite length_take min_l; first by eauto.
+    rewrite Hv. repeat unfold ly_size => /=; lia.
+  Qed.
+  Next Obligation. iIntros (??????[?[-> ?]]) "?". done. Qed.
+
+  Global Instance array_le : Proper ((=) ==> Forall2 (⊑) ==> (⊑)) array.
+  Proof.
+    move => ? sl -> tys1 tys2 Htys. constructor.
+    - move => β l; rewrite/ty_own/=.
+      f_equiv. f_equiv; first by rewrite ->Htys.
+      elim: Htys l => // ???????? /=. f_equiv; [solve_proper|].
+      by setoid_rewrite offset_loc_S.
+    - move => v; rewrite/ty_own_val/=.
+      f_equiv. { f_equiv; first by rewrite ->Htys. }
+      elim: Htys v => // ???? Hty Htys IH v /=. f_equiv. { solve_proper. }
+      apply: IH.
+  Qed.
+  Global Instance array_proper : Proper ((=) ==> Forall2 (≡) ==> (≡)) array.
+  Proof. move => ??-> ?? Heq. apply type_le_equiv_list; [by apply array_le|done]. Qed.
+
+  Global Instance array_loc_in_bounds ly β tys : LocInBounds (array ly tys) β (ly_size ly * length tys).
+  Proof. constructor. iIntros (?) "(?&$&?)". Qed.
+
+  Lemma array_get_type (i : nat) ly tys ty l β:
+    tys !! i = Some ty →
+    l ◁ₗ{β} array ly tys -∗ (l offset{ly}ₗ i) ◁ₗ{β} ty ∗ l ◁ₗ{β} array ly (<[ i := place (l offset{ly}ₗ i)]>tys).
+  Proof.
+    rewrite !/(ty_own (array _ _))/=. iIntros (Hi) "($&Hb&Ha)".
+    iInduction (i) as [|i] "IH" forall (l tys Hi);
+    destruct tys as [|ty' tys] => //; simpl in *; simplify_eq;
+    iDestruct "Ha" as "[$ Ha]".
+    { unfold place; by iFrame. }
+    rewrite offset_loc_S. setoid_rewrite offset_loc_S.
+    iDestruct (loc_in_bounds_split_mul_S with "Hb") as "[Hb1 Hb2]".
+    rewrite /offset_loc Z.mul_1_r.
+    iDestruct ("IH" with "[//] [Hb2] Ha") as "[$[Hb2 $]]" => //.
+    iApply loc_in_bounds_split_mul_S. iFrame.
+  Qed.
+
+  Lemma array_put_type (i : nat) ly tys ty l β:
+    (l offset{ly}ₗ i) ◁ₗ{β} ty -∗ l ◁ₗ{β} array ly tys -∗ l ◁ₗ{β} array ly (<[ i := ty ]>tys).
+  Proof.
+    rewrite !/(ty_own (array _ _))/=. iIntros "Hl ($&Hb&Ha)".
+    destruct (decide (i < length tys)%nat) as [Hlt |]; last first.
+    { rewrite list_insert_ge => //; last by lia. iFrame. }
+    iInduction (i) as [|i] "IH" forall (l tys Hlt);
+    destruct tys as [|ty' tys] => //; simpl in *; simplify_eq; eauto.
+    - iFrame. by iDestruct "Ha" as "[_ $]".
+    - rewrite offset_loc_S. setoid_rewrite offset_loc_S.
+      iDestruct "Ha" as "[$ Ha]".
+      iDestruct (loc_in_bounds_split_mul_S with "Hb") as "[Hb1 Hb2]".
+      rewrite /offset_loc Z.mul_1_r.
+      iDestruct ("IH" with "[] Hl [Hb2] Ha") as "[Hb2 $]" => //.
+      { iPureIntro. lia. }
+      iApply loc_in_bounds_split_mul_S. iFrame.
+  Qed.
+
+  Global Instance array_alloc_alive ly tys β P `{!TCExists (λ ty, AllocAlive ty β P) tys} :
+    AllocAlive (array ly tys) β P.
+  Proof.
+    revert select (TCExists _ _).
+    rewrite TCExists_Exists Exists_exists => -[x [/(elem_of_list_lookup_1 _ _) [i Hx] ?]].
+    constructor. iIntros (l) "HP Hl".
+    iDestruct (array_get_type with "Hl") as "[Hl _]"; [done|].
+    iDestruct (alloc_alive_alive with "HP Hl") as "Hl".
+    by iApply (alloc_alive_loc_mono with "Hl").
+  Qed.
+
+  Lemma subsume_array_alloc_alive A l ly tys β T :
+    (⌜0 < length tys⌝ ∗ (∀ ty, ⌜tys !! 0%nat = Some ty⌝ -∗ l ◁ₗ{β} ty -∗ alloc_alive_loc l ∗ ∃ x, T x))
+    ⊢ subsume (l ◁ₗ{β} array ly tys) (λ x : A, alloc_alive_loc l) T.
+  Proof.
+    iIntros "[% HT]". destruct tys => //=. iIntros "(%&?&[Hty Htys])".
+    rewrite offset_loc_0. iDestruct ("HT" with "[//] Hty") as "[? [% ?]]".
+    iExists _. iFrame.
+  Qed.
+  Definition subsume_array_alloc_alive_inst := [instance subsume_array_alloc_alive].
+  Global Existing Instance subsume_array_alloc_alive_inst | 10.
+  (*** array_ptr *)
+  Program Definition array_ptr (ly : layout) (base : loc) (idx : Z) (len : nat) : type := {|
+    ty_own β l := (
+      ⌜l = base offset{ly}ₗ idx⌝ ∗
+      ⌜l `has_layout_loc` ly⌝ ∗
+      ⌜0 ≤ idx ≤ len⌝ ∗
+      loc_in_bounds base (ly_size (mk_array_layout ly len))
+    )%I;
+    ty_has_op_type _ _ := False%type;
+    ty_own_val _ := True%I;
+  |}.
+  Solve Obligations with try done.
+  Next Obligation. iIntros (ly base idx len l E ?) "(%&%&$)". done. Qed.
+
+  Global Instance array_ptr_loc_in_bounds ly base idx β len : LocInBounds (array_ptr ly base idx len) β ((len - Z.to_nat idx) * ly_size ly).
+  Proof.
+    constructor. iIntros (?) "(->&%&%&Hl)".
+    iApply (loc_in_bounds_offset with "Hl") => /=; unfold addr in *; [done|lia|].
+    rewrite /mk_array_layout{3}/ly_size/=. nia.
+  Qed.
+  (*** typing rules *)
+
+  Lemma array_replicate_uninit_equiv l β ly n:
+    layout_wf ly →
+    l ◁ₗ{β} array ly (replicate n (uninit ly)) ⊣⊢ l ◁ₗ{β} uninit (mk_array_layout ly n).
+  Proof.
+    rewrite /ty_own/= => ?. iSplit.
+    - iInduction n as [|n] "IH" forall (l) => /=; iIntros "(%&Hlib&Htys)".
+      { iExists []. rewrite heap_mapsto_own_state_nil Nat.mul_0_r Forall_nil.
+        iFrame "Hlib". iPureIntro. rewrite /has_layout_val/ly_size/=. naive_solver lia. }
+      setoid_rewrite offset_loc_S. setoid_rewrite offset_loc_1. rewrite offset_loc_0.
+      iDestruct "Htys" as "[Hty Htys]".
+      iDestruct (loc_in_bounds_split_mul_S with "Hlib") as "[#Hlib1 Hlib2]".
+      iDestruct ("IH" with "[Hlib2 Htys]") as (v2 Hv2 ? _) "Hv2".
+      { iFrame. iPureIntro. revert select (layout_wf _). revert select (_ `has_layout_loc` _).
+        rewrite /has_layout_loc /layout_wf /aligned_to. case_match => //. destruct l as [? a].
+        move => /= [? ->] [? ->]. eexists. by rewrite -Z.mul_add_distr_r. }
+      rewrite {2}/ty_own/=. iDestruct "Hty" as (v1 Hv1 Hl1 _) "Hv1".
+      iExists (v1 ++ v2). rewrite heap_mapsto_own_state_app Hv1 /has_layout_val length_app Hv1 Hv2.
+      iFrame. rewrite Forall_forall. iPureIntro. split_and! => //.
+      rewrite {2 3}/ly_size/=. lia.
+    - iDestruct 1 as (v Hv Hl _) "Hl". iSplit => //.
+      iInduction n as [|n] "IH" forall (v l Hv Hl) => /=.
+      { rewrite Nat.mul_0_r right_id.
+        iApply loc_in_bounds_shorten; last by iApply heap_mapsto_own_state_loc_in_bounds. lia. }
+      setoid_rewrite offset_loc_S. setoid_rewrite offset_loc_1. rewrite offset_loc_0.
+      rewrite -(take_drop (ly.(ly_size)) v) heap_mapsto_own_state_app.
+      iDestruct "Hl" as "[Hl Hr]". rewrite length_take_le ?Hv; last by repeat unfold ly_size => /=; lia.
+      iDestruct (heap_mapsto_own_state_loc_in_bounds with "Hl") as "#Hbl".
+      iDestruct (heap_mapsto_own_state_loc_in_bounds with "Hr") as "#Hbr".
+      iDestruct ("IH" with "[] [] Hr") as "[Hb HH]".
+      { iPureIntro. rewrite /has_layout_val length_drop Hv. repeat unfold ly_size => /=; lia. }
+      { iPureIntro. by apply has_layout_loc_ly_mult_offset. }
+      iSplitR.
+      + iClear "IH". iApply loc_in_bounds_split_mul_S.
+        rewrite length_take min_l; last first.
+        { rewrite Hv. repeat unfold ly_size => /=; lia. }
+        iFrame "Hbl". rewrite length_replicate length_drop Hv.
+        destruct ly as [k?]. repeat unfold ly_size => /=.
+        have ->: (k * n = k * S n - k)%nat by lia. done.
+      + iSplitL "Hl"; last done. iExists _. iFrame. iPureIntro. rewrite Forall_forall. split_and! => //.
+        rewrite /has_layout_val length_take_le ?Hv; repeat unfold ly_size => /=; lia.
+  Qed.
+
+  Lemma simplify_hyp_uninit_array ly l β n T:
+    ⌜layout_wf ly⌝ ∗ (l ◁ₗ{β} array ly (replicate n (uninit ly)) -∗ T)
+    ⊢ simplify_hyp (l ◁ₗ{β} uninit (mk_array_layout ly n)) T.
+  Proof. iIntros "[% HT] Hl". iApply "HT". rewrite array_replicate_uninit_equiv // {1}/ly_size/=. Qed.
+  Definition simplify_hyp_uninit_array_inst := [instance simplify_hyp_uninit_array with 50%N].
+  Global Existing Instance simplify_hyp_uninit_array_inst.
+
+  Lemma simplify_goal_uninit_array ly l β n T:
+    ⌜layout_wf ly⌝ ∗ l ◁ₗ{β} array ly (replicate n (uninit ly)) ∗ T
+    ⊢ simplify_goal (l ◁ₗ{β} uninit (mk_array_layout ly n)) T.
+  Proof. iIntros "[% [? $]]". rewrite array_replicate_uninit_equiv //. Qed.
+  Definition simplify_goal_uninit_array_inst := [instance simplify_goal_uninit_array with 50%N].
+  Global Existing Instance simplify_goal_uninit_array_inst.
+
+  (* TODO: generalize this rule, maybe similar to [subsume_array_uninit]? *)
+  Lemma subsume_uninit_array_replicate A l β n (ly1 : layout) ly2 T:
+    (∃ x, ⌜layout_wf ly2⌝ ∗ ⌜ly1 = mk_array_layout ly2 n⌝ ∗ T x)
+    ⊢ subsume (l ◁ₗ{β} uninit ly1) (λ x : A, l ◁ₗ{β} array ly2 (replicate n (uninit ly2))) T.
+  Proof. iIntros "(%&%&->&?) ?". iExists _. iFrame. by rewrite array_replicate_uninit_equiv. Qed.
+  Definition subsume_uninit_array_replicate_inst := [instance subsume_uninit_array_replicate].
+  Global Existing Instance subsume_uninit_array_replicate_inst.
+
+  Lemma subsume_array_uninit A l β tys ly1 ly2 T:
+    (l ◁ₗ{β} array ly2 tys -∗
+      ⌜layout_wf ly2⌝ ∗ l ◁ₗ{β} array ly2 (replicate (length tys) (uninit ly2)) ∗
+      ∃ x, ⌜ly1 x = mk_array_layout ly2 (length tys)⌝ ∗ T x)
+    ⊢ subsume (l ◁ₗ{β} array ly2 tys) (λ x : A, l ◁ₗ{β} uninit (ly1 x)) T.
+  Proof.
+    iIntros "Hsub ?". iDestruct ("Hsub" with "[$]") as (?) "[? [% [%Heq ?]]]".
+    iExists _. iFrame. by rewrite Heq array_replicate_uninit_equiv.
+  Qed.
+  Definition subsume_array_uninit_inst := [instance subsume_array_uninit].
+  Global Existing Instance subsume_array_uninit_inst.
+
+  Lemma subsume_array A ly1 ly2 tys1 tys2 l β T:
+    (⌜ly1 = ly2⌝ ∗ ∀ id,
+       subsume (sep_list id type [] tys1 (λ i ty, (l offset{ly1}ₗ i) ◁ₗ{β} ty))
+         (λ x, sep_list id type [] (tys2 x) (λ i ty, (l offset{ly1}ₗ i) ◁ₗ{β} ty)) T)
+    ⊢ subsume (l ◁ₗ{β} array ly1 tys1) (λ x : A, l ◁ₗ{β} array ly2 (tys2 x)) T.
+  Proof.
+    unfold sep_list. iIntros "[-> H] ($&Hb&H1)".
+    iDestruct ("H" $! {|sep_list_len := length tys1|} with "[$H1]") as (?) "[[%Heq ?] ?]"; [done|].
+    simpl in *. rewrite -Heq. iExists _. iFrame.
+  Qed.
+  Definition subsume_array_inst := [instance subsume_array].
+  Global Existing Instance subsume_array_inst.
+
+  Lemma type_place_array l β ly1 it v tyv tys ly2 K T:
+    (v ◁ᵥ tyv -∗ ∃ i, ⌜ly1 = ly2⌝ ∗ v ◁ᵥ i @ int it ∗ ⌜0 ≤ i⌝ ∗ ⌜i < length tys⌝ ∗
+     ∀ ty, ⌜tys !! Z.to_nat i = Some ty⌝ -∗
+      typed_place K (l offset{ly2}ₗ i) β ty (λ l2 β2 ty2 typ,
+       T l2 β2 ty2 (λ t, array ly2 (<[Z.to_nat i := typ t]>tys))))
+    ⊢ typed_place (BinOpPCtx (PtrOffsetOp ly1) (IntOp it) v tyv :: K) l β (array ly2 tys) T.
+  Proof.
+    iIntros "HT" (Φ) "(%&#Hb&Hl) HΦ" => /=. iIntros "Hv".
+    iDestruct ("HT" with "Hv") as (i ->) "HP". unfold int; simpl_type.
+    iDestruct ("HP") as (Hv) "HP".
+    iDestruct "HP" as (? Hlen) "HP".
+    have [|ty ?]:= lookup_lt_is_Some_2 tys (Z.to_nat i). 1: lia.
+    iApply wp_ptr_offset => //; [by apply val_to_of_loc | | ].
+    { iApply (loc_in_bounds_offset with "Hb"); simpl; [done| destruct l => /=; lia | destruct l => /=; nia]. }
+    iIntros "!#". iExists _. iSplit => //.
+    iDestruct (big_sepL_insert_acc with "Hl") as "[Hl Hc]" => //. rewrite Z2Nat.id//.
+    iApply ("HP" $! ty with "[//] Hl"). iIntros (l' ty2 β2 typ R) "Hl' Htyp HT".
+    iApply ("HΦ" with "Hl' [-HT] HT"). iIntros (ty') "Hl'".
+    iMod ("Htyp" with "Hl'") as "[? $]".
+    iSplitR => //. iSplitR; first by rewrite length_insert. by iApply "Hc".
+  Qed.
+  Definition type_place_array_inst := [instance type_place_array].
+  Global Existing Instance type_place_array_inst.
+
+  Lemma type_bin_op_offset_array l β ly it v tys i T:
+    (* TODO: Should we make layout_wf ly part of array such that we don't need to require it here? *)
+    ⌜layout_wf ly⌝ ∗ ⌜0 ≤ i ≤ length tys⌝ ∗ (l ◁ₗ{β} array ly tys -∗ T (val_of_loc (l offset{ly}ₗ i)) ((l offset{ly}ₗ i) @ &own (array_ptr ly l i (length tys))))
+    ⊢ typed_bin_op v (v ◁ᵥ i @ int it) l (l ◁ₗ{β} array ly tys) (PtrOffsetOp ly) (IntOp it) PtrOp T.
+  Proof.
+    iIntros "[% [% HT]]". unfold int; simpl_type.
+    iIntros "%Hv (%&#Hlib&Hl)" (Φ) "HΦ".
+    iApply wp_ptr_offset => //; [by apply val_to_of_loc | | ].
+    { iApply (loc_in_bounds_offset with "Hlib"); simpl; [done| destruct l => /=; lia | destruct l => /=; nia]. }
+    iModIntro. iApply "HΦ"; [|iApply "HT"; iFrame; by iSplit].
+    unfold frac_ptr; simpl_type. iSplit; [done|]. iSplit; [done|].
+    iSplit; [| by iSplit].
+    iPureIntro. by apply: has_layout_loc_offset_loc.
+  Qed.
+  Definition type_bin_op_offset_array_inst := [instance type_bin_op_offset_array].
+  Global Existing Instance type_bin_op_offset_array_inst.
+
+  Lemma type_bin_op_offset_array_ptr l β ly it v i idx (len : nat) base T:
+    ⌜layout_wf ly⌝ ∗ ⌜0 ≤ idx + i ≤ len⌝ ∗ (l ◁ₗ{β} array_ptr ly base idx len -∗ T (val_of_loc (base offset{ly}ₗ (idx + i))) ((base offset{ly}ₗ (idx + i)) @ &own (array_ptr ly base (idx + i) len)))
+    ⊢ typed_bin_op v (v ◁ᵥ i @ int it) l (l ◁ₗ{β} array_ptr ly base idx len) (PtrOffsetOp ly) (IntOp it) PtrOp T.
+  Proof.
+    iIntros "[% [% HT]]". unfold int; simpl_type.
+    iIntros "%Hv (->&%&%&#Hlib)" (Φ) "HΦ".
+    iApply wp_ptr_offset => //; [by apply val_to_of_loc | | ].
+    { iApply (loc_in_bounds_offset with "Hlib"); simpl; unfold addr in *; [done|nia|].
+      rewrite {3}/ly_size/=. nia. }
+    rewrite offset_loc_offset_loc.
+    iModIntro. iApply "HΦ"; [|iApply "HT"]; unfold frac_ptr; simpl_type; iFrame "Hlib"; iPureIntro; [|done].
+    split_and! => //; try lia. rewrite -offset_loc_offset_loc.
+    by apply has_layout_loc_offset_loc.
+  Qed.
+  Definition type_bin_op_offset_array_ptr_inst := [instance type_bin_op_offset_array_ptr].
+  Global Existing Instance type_bin_op_offset_array_ptr_inst.
+
+  Lemma type_bin_op_neg_offset_array_ptr l β ly it v i idx (len : nat) base T:
+    ⌜layout_wf ly⌝ ∗ ⌜0 ≤ idx - i ≤ len⌝ ∗ (l ◁ₗ{β} array_ptr ly base idx len -∗ T (val_of_loc (base offset{ly}ₗ (idx - i))) ((base offset{ly}ₗ (idx - i)) @ &own (array_ptr ly base (idx - i) len)))
+    ⊢ typed_bin_op v (v ◁ᵥ i @ int it) l (l ◁ₗ{β} array_ptr ly base idx len) (PtrNegOffsetOp ly) (IntOp it) PtrOp T.
+  Proof.
+    iIntros "[% [% HT]]". unfold int; simpl_type.
+    iIntros "%Hv (->&%&%&#Hlib)" (Φ) "HΦ".
+    iApply wp_ptr_neg_offset => //; [by apply val_to_of_loc | | ].
+    { iApply (loc_in_bounds_offset with "Hlib"); simpl; unfold addr in *; [done|nia|].
+      rewrite {3}/ly_size/=. nia. }
+    rewrite offset_loc_offset_loc Z.add_opp_r.
+    iModIntro. iApply "HΦ"; [|iApply "HT"]; unfold frac_ptr; simpl_type; iFrame "Hlib"; iPureIntro; [|done].
+    split_and! => //; try lia. rewrite -Z.add_opp_r -offset_loc_offset_loc.
+    by apply has_layout_loc_offset_loc.
+  Qed.
+  Definition type_bin_op_neg_offset_array_ptr_inst := [instance type_bin_op_neg_offset_array_ptr].
+  Global Existing Instance type_bin_op_neg_offset_array_ptr_inst.
+
+  Lemma type_bin_op_diff_array_ptr_array l1 β l2 ly idx (len : nat) tys T:
+    (l1 ◁ₗ{β} array_ptr ly l2 idx len -∗
+    l2 ◁ₗ{β} array ly tys -∗
+    ⌜0 < ly.(ly_size)⌝ ∗
+    ⌜0 < length tys⌝ ∗
+    ⌜idx ≤ max_int ptrdiff_t⌝ ∗
+    (alloc_alive_loc l2 ∗ True) ∧
+    (T (i2v idx ptrdiff_t) (idx @ int ptrdiff_t)))
+    ⊢ typed_bin_op l1 (l1 ◁ₗ{β} array_ptr ly l2 idx len) l2 (l2 ◁ₗ{β} array ly tys) (PtrDiffOp ly) PtrOp PtrOp T.
+  Proof.
+    iIntros "HT (->&%&%&#Hlib) Hl2" (Φ) "HΦ".
+    iDestruct ("HT" with "[$Hlib//] Hl2") as (? ? ?) "HT".
+    have /(val_of_Z_is_Some None) [vo Hvo] : idx ∈ ptrdiff_t. {
+      split; [|done].
+      rewrite /min_int/=/int_half_modulus/=/bits_per_int/bytes_per_int/=/bits_per_byte. lia.
+    }
+    rewrite /i2v Hvo/=.
+    iApply wp_ptr_diff; [by apply: val_to_of_loc|by apply: val_to_of_loc| |done|done| | |].
+    { rewrite /= Z.add_simpl_l Z.mul_comm Z.div_mul //. lia. }
+    { iApply (loc_in_bounds_offset with "Hlib"); simpl; unfold addr in *; [done|nia|].
+      rewrite {2}/ly_size/=. nia. }
+    { iApply (loc_in_bounds_shorten with "Hlib"). lia. }
+    iSplit. {
+      iApply alloc_alive_loc_mono; [simpl; done|].
+      iDestruct "HT" as "[[$ _] _]".
+    }
+    iDestruct "HT" as "[_ HT]".
+    iModIntro. iApply "HΦ"; [|iApply "HT"].
+    unfold int; simpl_type. iPureIntro. by apply: val_to_of_Z.
+  Qed.
+  Definition type_bin_op_diff_array_ptr_array_inst := [instance type_bin_op_diff_array_ptr_array].
+  Global Existing Instance type_bin_op_diff_array_ptr_array_inst.
+
+  Lemma subsume_array_ptr_alloc_alive A β l ly base idx len T:
+    (alloc_alive_loc base ∗ ∃ x, T x)
+    ⊢ subsume (l ◁ₗ{β} array_ptr ly base idx len) (λ x : A, alloc_alive_loc l) T.
+  Proof.
+    iIntros "[Halive [% ?]] (->&?)".
+    iExists _. iFrame. by iApply (alloc_alive_loc_mono with "Halive").
+  Qed.
+  Definition subsume_array_ptr_alloc_alive_inst := [instance subsume_array_ptr_alloc_alive].
+  Global Existing Instance subsume_array_ptr_alloc_alive_inst | 10.
+
+  Lemma simpl_goal_array_ptr ly base idx1 idx2 len β T:
+    ⌜idx1 = idx2⌝ ∗ ⌜(base offset{ly}ₗ idx1) `has_layout_loc` ly⌝ ∗ ⌜0 ≤ idx1 ≤ Z.of_nat len⌝ ∗
+       loc_in_bounds base (ly_size (mk_array_layout ly len)) ∗ T
+    ⊢ simplify_goal ((base offset{ly}ₗ idx1) ◁ₗ{β} array_ptr ly base idx2 len)  T.
+  Proof. by iIntros "(->&%&%&$&$)". Qed.
+  Definition simpl_goal_array_ptr_inst := [instance simpl_goal_array_ptr with 50%N].
+  Global Existing Instance simpl_goal_array_ptr_inst.
+
+  Lemma subsume_array_ptr A ly1 ly2 base1 base2 idx1 idx2 len1 len2 l β T:
+    (∃ x, ⌜ly1 = ly2 x⌝ ∗ ⌜base1 = base2 x⌝ ∗ ⌜idx1 = idx2 x⌝ ∗ ⌜len1 = len2 x⌝ ∗ T x)
+    ⊢ subsume (l ◁ₗ{β} array_ptr ly1 base1 idx1 len1)
+        (λ x : A, l ◁ₗ{β} array_ptr (ly2 x) (base2 x) (idx2 x) (len2 x)) T.
+  Proof. iIntros "(%&->&->&->&->&?) ?". iExists _. iFrame. Qed.
+  Definition subsume_array_ptr_inst := [instance subsume_array_ptr].
+  Global Existing Instance subsume_array_ptr_inst.
+
+  (*
+  TODO: The following rule easily leads to diverging if the hypothesis is simplified before it is introduced into the context.
+  Lemma simplify_array_ptr_hyp_learn_loc l β ly base idx len T:
+    (⌜l = base offset{ly}ₗ idx⌝ -∗ l ◁ₗ{β} array_ptr ly base idx len -∗ T
+    ⊢ simplify_hyp (l ◁ₗ{β} array_ptr ly base idx len) T.
+  Proof. iIntros "HT [% #Hlib]". iApply "HT" => //. by iSplit. Qed.
+  Global Instance simplify_array_ptr_hyp_learn_loc_inst l β ly base idx len `{!TCUnless (TCFastDone (l = base offset{ly}ₗ idx))}:
+    SimplifyHyp _ (Some 0%N) | 10 :=
+    λ T, i2p (simplify_array_ptr_hyp_learn_loc l β ly base idx len T).
+*)
+
+  Lemma simplify_hyp_array_ptr ly l β base idx len T:
+    (⌜l = (base offset{ly}ₗ idx)⌝ -∗
+    ⌜(base offset{ly}ₗ idx) `has_layout_loc` ly⌝ -∗
+    loc_in_bounds base (ly_size (mk_array_layout ly len)) -∗
+    ∃ tys, base ◁ₗ{β} array ly tys ∗ ⌜0 ≤ idx < length tys⌝ ∗ (
+      ∀ ty, ⌜tys !! Z.to_nat idx = Some ty⌝ -∗ base ◁ₗ{β} array ly (<[Z.to_nat idx := place l]>tys) -∗
+        l ◁ₗ{β} ty -∗ T))
+    ⊢ simplify_hyp (l ◁ₗ{β} array_ptr ly base idx len) T.
+  Proof.
+    iIntros "HT (->&%&%&?)".
+    iDestruct ("HT" with "[//] [//] [$]") as (tys) "(Harray&%&HT)".
+    have [|ty ?]:= lookup_lt_is_Some_2 tys (Z.to_nat idx). 1: lia.
+    iDestruct (array_get_type (Z.to_nat idx) with "Harray") as "[Hty Harray]"; [done|].
+    rewrite Z2Nat.id; [|lia].
+    by iApply ("HT" with "[//] Harray Hty").
+  Qed.
+  Definition simplify_hyp_array_ptr_inst := [instance simplify_hyp_array_ptr with 50%N].
+  Global Existing Instance simplify_hyp_array_ptr_inst | 50.
+End array.
+
+Notation "array< ty , tys >" := (array ty tys)
+  (only printing, format "'array<' ty ,  tys '>'") : printing_sugar.
+Global Typeclasses Opaque array.
+Global Typeclasses Opaque array_ptr.
